progress on traces

IMP/HOL_TCN_Timing.thy
@@ -1,6 +1,9 @@
 theory HOL_TCN_Timing
-  imports "HOL-Library.Log_Nat" IMP_Tailcall Fresh
+  imports Com
 begin
+
+unbundle no com_syntax
+declare [[syntax_ambiguity_warning=false]]
 
 (* general stuff *)
 
@@ -28,6 +31,17 @@ notation hLet ("LET _ IN _") and
          hIf ("(IF _/\<noteq>0 THEN _/ ELSE _)"  [0, 0, 61] 61)
 end
 
+
+fun calls where
+  "calls (LET t1 IN t2) = calls t1 @ calls t2" |
+  "calls (hLetBound _) = []" |
+  "calls (hArg _) = []" |
+  "calls (hNumber _) = []" |
+  "calls (IF t1\<noteq>0 THEN t2 ELSE t3) = calls t1 @ calls t2 @ calls t3" |
+  "calls (hCall f ts) = f # concat (map calls ts)" |
+  "calls (hTAIL ts) = concat (map calls ts)"
+
+
 (* function name \<Rightarrow> (function \<times> timing function) *)
 type_synonym thol_reg = "fun_ref \<Rightarrow> ((nat list \<Rightarrow> nat) \<times> (nat list \<Rightarrow> nat))"
 abbreviation "f_from_reg (reg :: thol_reg) name \<equiv> fst (reg name)"
@@ -46,7 +60,6 @@ abbreviation "ret_from_ctxt (ctxt :: thol_ctxt) name \<equiv> snd (snd (ctxt nam
 (* TODO: use better names than reg/ctxt *)
 
 definition "null = (\<lambda>_. undefined)"
-
 
 
 inductive
@@ -71,34 +84,6 @@ hTAIL: "\<lbrakk>length zs = length ts; length vs = length ts;
           z'' = sum_list zs + z' + 1\<rbrakk>
           \<Longrightarrow> (f,reg) \<turnstile> (hTAIL ts,bs,xs) \<Rightarrow>\<^bsup>z''\<^esup> v'"
 
-
-
-
-(* 
-(* TODO: use list_all instead of quantifiers?:
-    list_all (\<lambda>(ti, zi, vi). (f,reg) \<turnstile> (ti,bs,xs) \<Rightarrow>\<^bsup>zi\<^esup> vi) (zip ts (zip zs vs)) *)
-inductive
-  hbig_step_t :: "thol \<times> thol_reg \<Rightarrow> thol \<times> nat list \<times> nat list \<Rightarrow> nat \<Rightarrow> nat \<Rightarrow> bool" ("_ \<turnstile> _ \<Rightarrow>\<^bsup>_\<^esup>  _" 55)
-  where
-hLet: "\<lbrakk>env \<turnstile> (t1,bs,xs) \<Rightarrow>\<^bsup>z1\<^esup> v1; env \<turnstile> (t2,v1#bs,xs) \<Rightarrow>\<^bsup>z2\<^esup> v; z = z1+z2\<rbrakk>
-       \<Longrightarrow> env \<turnstile> (hLet t1 t2,bs,xs) \<Rightarrow>\<^bsup>z\<^esup> v" |
-hLetBound: "v = bs!n \<Longrightarrow> env \<turnstile> (hLetBound n,bs,xs) \<Rightarrow>\<^bsup>0\<^esup> v" |
-hArg: "v = xs!n \<Longrightarrow> env \<turnstile> (hArg n,bs,xs) \<Rightarrow>\<^bsup>0\<^esup> v" |
-hNumber: "env \<turnstile> (hNumber n,bs,xs) \<Rightarrow>\<^bsup>0\<^esup> n" |
-hIfTrue: "\<lbrakk>env \<turnstile> (t1,bs,xs) \<Rightarrow>\<^bsup>z1\<^esup> v1; v1 \<noteq> 0; env \<turnstile> (t2,bs,xs) \<Rightarrow>\<^bsup>z2\<^esup> v2; z = z1+z2\<rbrakk>
-          \<Longrightarrow> env \<turnstile> (hIf t1 t2 t3,bs,xs) \<Rightarrow>\<^bsup>z\<^esup> v2" |
-hIfFalse: "\<lbrakk>env \<turnstile> (t1,bs,xs) \<Rightarrow>\<^bsup>z1\<^esup> v1; v1 = 0; env \<turnstile> (t3,bs,xs) \<Rightarrow>\<^bsup>z2\<^esup> v2; z = z1+z2\<rbrakk>
-          \<Longrightarrow> env \<turnstile> (hIf t1 t2 t3,bs,xs) \<Rightarrow>\<^bsup>z\<^esup> v2" |
-hCall: "\<lbrakk>reg vg = (g, T_g); length zs = length ts; length vs = length ts;
-          \<And>ti vi zi. (ti, zi, vi) \<in> set (zip ts (zip zs vs)) \<longrightarrow> (f,reg) \<turnstile> (ti,bs,xs) \<Rightarrow>\<^bsup>zi\<^esup> vi;
-          g vs = v'; z' = sum_list zs + T_g vs\<rbrakk>
-          \<Longrightarrow> (f,reg) \<turnstile> (hCall vg ts,bs,xs) \<Rightarrow>\<^bsup>z'\<^esup> v'" |
-hTAIL: "\<lbrakk>length zs = length ts; length vs = length ts;
-          \<And>ti vi zi. (ti, zi, vi) \<in> set (zip ts (zip zs vs)) \<longrightarrow> (f,reg) \<turnstile> (ti,bs,xs) \<Rightarrow>\<^bsup>zi\<^esup> vi;
-          (f,reg) \<turnstile> (f,[],vs) \<Rightarrow>\<^bsup>z'\<^esup> v';
-          z'' = sum_list zs + z' + 1\<rbrakk>
-          \<Longrightarrow> (f,reg) \<turnstile> (hTAIL ts,bs,xs) \<Rightarrow>\<^bsup>z''\<^esup> v'" *)
-
 print_theorems
 
 (* code_pred [show_modes] hbig_step_t . (* can't handle the universal quantifier *) *)
@@ -120,7 +105,7 @@ lemma determ:
   assumes "ctxt \<turnstile> (t,bs,xs) \<Rightarrow>\<^bsup>z1\<^esup> v1"
   assumes "ctxt \<turnstile> (t,bs,xs) \<Rightarrow>\<^bsup>z2\<^esup> v2"
   shows "z1 = z2" "v1 = v2"
-  oops
+  oops (* TODO *)
 (* using assms proof (induction arbitrary: z2 v2 rule: hbig_step_t.induct)
   case (hCall g T_g reg gr zs ts vs f bs xs v' z')
   {
@@ -156,7 +141,7 @@ fun invar where
   "invar (hTAIL ts) = (\<forall>t \<in> set ts. \<not> tails t)" |
   "invar _ = True"
 
-lemma non_tail_invar[simp]: "\<not> tails t \<Longrightarrow> invar t" by (induction t) auto
+lemma no_tails_invar[simp]: "\<not> tails t \<Longrightarrow> invar t" by (induction t) auto
 
 
 (* traces *)
@@ -172,8 +157,6 @@ lemma interp_trace_append[simp]:
 lemma interp_trace_concat_is_sum_map:
   "interp_trace reg (concat xss) = sum_map (interp_trace reg) xss"
   unfolding interp_trace_def by (induction xss) auto
-
-
 
 datatype leaf_state = Value nat | Tail "nat list"
 
@@ -206,9 +189,31 @@ hTail:
 lemmas htrace_to_leaf_induct = htrace_to_leaf.induct[split_format(complete)]
 
 
-(* relating traces to the semantics *)
+(* relating traces to the semantics
 
-lemma trace_non_tail0:
+For any t/bs/xs, there are two cases depending on whether t runs to Value or to Tail:
+
+Case 1:
+  |----- Value v|  (trace)
+  |----------- v|  (sem.)
+
+Case 2:
+  |---- Tail xs'||----------- v|  (trace, sem.)
+  |-------------------------- v|  (sem.)
+
+In the direction trace \<longrightarrow> semantics:
+- For case 1, we show: if there is a trace, there is a corresponding inference in the semantics.
+- For case 2, we show: if there is a trace to Tail xs' and an inference in the semantics from f/[]/xs',
+  there is a corresponding inference in the semantics for the "whole execution" from t/bs/xs.
+
+In the direction semantics \<longrightarrow> trace:
+We show: if there is a semantics, either:
+- there exists a corresponding trace to a value (i.e. no tail call occurs), or
+- there exists a trace to Tail xs', and from f/[]/xs' a semantics to a value.
+
+*)
+
+lemma trace_val_to_semantics0:
   assumes "reg \<turnstile> (t,bs,xs) \<Rightarrow>\<^bsup>(T :: trace)\<^esup> l" "l = Value v"
   shows "(f,reg) \<turnstile> (t,bs,xs) \<Rightarrow>\<^bsup> interp_trace reg T \<^esup> v"
 using assms proof (induction arbitrary: v rule: htrace_to_leaf_induct)
@@ -225,13 +230,13 @@ using assms proof (induction arbitrary: v rule: htrace_to_leaf_induct)
   qed (simp_all add: hCall)
 qed (simp_all add: interp_trace_def hbig_step_t.intros)
 
-theorem trace_non_tail:
+theorem trace_val_to_semantics:
   assumes "reg \<turnstile> (t,bs,xs) \<Rightarrow>\<^bsup>T\<^esup> Value v"
   shows "(f,reg) \<turnstile> (t,bs,xs) \<Rightarrow>\<^bsup> interp_trace reg T \<^esup> v"
-  using assms trace_non_tail0 by blast
+  using assms trace_val_to_semantics0 by blast
 
 
-lemma trace_tail0:
+lemma trace_tail_to_semantics0:
   assumes "reg \<turnstile> (t,bs,xs) \<Rightarrow>\<^bsup>(T :: trace)\<^esup> l" "l = Tail xs'"
   assumes "invar t"
   assumes "(f,reg) \<turnstile> (f,[],xs') \<Rightarrow>\<^bsup>z\<^esup> v"
@@ -245,7 +250,7 @@ using assms proof (induction arbitrary: rule: htrace_to_leaf_induct)
       using hLet interp_trace_append by simp
   next
     show "(f, reg) \<turnstile> (t1, bs, xs) \<Rightarrow>\<^bsup>interp_trace reg T1\<^esup> v1"
-      using hLet trace_non_tail by simp
+      using hLet trace_val_to_semantics by simp
   next
     show "(f, reg) \<turnstile> (t2, v1 # bs, xs) \<Rightarrow>\<^bsup>interp_trace reg T2 + z + 1\<^esup>  v"
       using hLet by simp
@@ -255,7 +260,7 @@ next
   show ?case
   proof (rule hbig_step_t.hIfTrue)
     show "(f, reg) \<turnstile> (t1, bs, xs) \<Rightarrow>\<^bsup>interp_trace reg T1\<^esup> v1"
-      using hIfTrue trace_non_tail by simp
+      using hIfTrue trace_val_to_semantics by simp
   next
     show "v1 \<noteq> 0" using hIfTrue by simp
   next
@@ -269,7 +274,7 @@ next
   show ?case
   proof (rule hbig_step_t.hIfFalse)
     show "(f, reg) \<turnstile> (t1, bs, xs) \<Rightarrow>\<^bsup>interp_trace reg T1\<^esup> v1"
-      using hIfFalse trace_non_tail by simp
+      using hIfFalse trace_val_to_semantics by simp
   next
     show "v1 = 0" using hIfFalse by simp
   next
@@ -286,409 +291,194 @@ next
     show "interp_trace reg T + z + 1 = sum_list ?zs + z + 1"
       using hTail interp_trace_concat_is_sum_map interp_trace_append by simp
   next show "\<forall>i<length ts. (f, reg) \<turnstile> (ts ! i, bs, xs) \<Rightarrow>\<^bsup>?zs ! i\<^esup> vs ! i"
-      using hTail[simplified] nth_map trace_non_tail by simp
+      using hTail[simplified] nth_map trace_val_to_semantics by simp
   next show "length vs = length ts" using hTail by simp
   next show "(f, reg) \<turnstile> (f, [], vs) \<Rightarrow>\<^bsup>z\<^esup> v" using hTail by simp
   next show "length (map (interp_trace reg) Ts) = length ts" using hTail by simp
   qed
 qed simp_all
 
-theorem trace_tail:
+theorem trace_tail_to_semantics:
   assumes "invar t"
   assumes "reg \<turnstile> (t,bs,xs) \<Rightarrow>\<^bsup>T\<^esup> Tail xs'"
   assumes "(f,reg) \<turnstile> (f,[],xs') \<Rightarrow>\<^bsup>z\<^esup> v"
   shows "(f,reg) \<turnstile> (t,bs,xs) \<Rightarrow>\<^bsup> interp_trace reg T + z + 1 \<^esup> v"
-  using assms trace_tail0 by blast
+  using assms trace_tail_to_semantics0 by blast
 
 
-(* lemma trace_exists:
+(* semantics \<longrightarrow> trace *)
+
+
+lemma sem_to_trace_non_tailE:
+  assumes "\<not> tails t"
   assumes "(f,reg) \<turnstile> (t,bs,xs) \<Rightarrow>\<^bsup> z \<^esup> v"
-  assumes "invar t"
-  shows "\<exists>(T :: trace) l. reg \<turnstile> (t,bs,xs) \<Rightarrow>\<^bsup>T\<^esup> l"
-  sorry *)
+  obtains T :: trace where "reg \<turnstile> (t,bs,xs) \<Rightarrow>\<^bsup>T\<^esup> Value v" "interp_trace reg T = z"
+  using assms(2,1) apply (induction rule: hbig_step_t_induct)
+  apply (metis HOL_TCN_Timing.tails.simps(2) htrace_to_leaf.hLet interp_trace_append)
+  apply (metis htrace_to_leaf.hLetBound interp_trace_def list.map(1) sum_list.Nil)
+  apply (metis htrace_to_leaf.hArg interp_trace_def list.map(1) sum_list.Nil)
+  apply (metis htrace_to_leaf.hNumber interp_trace_def list.map(1) sum_list.Nil)
+  apply (metis HOL_TCN_Timing.tails.simps(3) htrace_to_leaf.hIfTrue interp_trace_append)
+  apply (metis HOL_TCN_Timing.tails.simps(3) htrace_to_leaf.hIfFalse interp_trace_append)
+  sorry (* TODO *)
 
-lemma
+lemma sem_to_trace_inductionI:
+  assumes "P' \<or> (\<exists>xs'. Q1' xs' \<and> Q2' xs')"
+  assumes "P' \<Longrightarrow> P T"
+  assumes "\<And>xs'. Q1' xs' \<Longrightarrow> Q1 T xs'"
+  assumes "\<And>xs'. Q2' xs' \<Longrightarrow> Q2 T xs'"
+  shows "\<exists>T. P T \<or> (\<exists>xs'. Q1 T xs' \<and> Q2 T xs')"
+  using assms by blast
+
+lemma sem_to_traceE:
+  assumes "invar t"
+  assumes "(f,reg) \<turnstile> (t,bs,xs) \<Rightarrow>\<^bsup>z\<^esup> v"
+  shows "\<exists>T.
+    (reg \<turnstile> (t,bs,xs) \<Rightarrow>\<^bsup>T\<^esup> Value v) \<or>
+    (\<exists>xs'. reg \<turnstile> (t,bs,xs) \<Rightarrow>\<^bsup>T\<^esup> Tail xs'
+           \<and> (f,reg) \<turnstile> (f,[],xs') \<Rightarrow>\<^bsup>z - interp_trace reg T - 1\<^esup> v)"
+using assms(2,1) proof (induction rule: hbig_step_t_induct)
+  case (hLet f reg t1 bs xs z1 v1 t2 z2 v z)
+
+  from sem_to_trace_non_tailE hLet.hyps(1) obtain T1 where
+    T1: "reg \<turnstile> (t1,bs,xs) \<Rightarrow>\<^bsup>T1\<^esup> Value v1" "interp_trace reg T1 = z1"
+    using hLet.prems invar.simps by blast
+  from hLet.IH(2) obtain T2 where
+      "(reg \<turnstile> (t2,v1#bs,xs) \<Rightarrow>\<^bsup>T2\<^esup> Value v) \<or>
+       (\<exists>xs'. reg \<turnstile> (t2,v1#bs,xs) \<Rightarrow>\<^bsup>T2\<^esup> Tail xs' \<and>
+              (f, reg) \<turnstile> (f,[],xs') \<Rightarrow>\<^bsup>z2 - interp_trace reg T2 - 1\<^esup> v)"
+    using hLet.prems by auto
+  then show ?case proof (rule sem_to_trace_inductionI)
+    assume "reg \<turnstile> (t2,v1#bs,xs) \<Rightarrow>\<^bsup>T2\<^esup> Value v"
+    then show "reg \<turnstile> (LET t1 IN t2,bs,xs) \<Rightarrow>\<^bsup>T1@T2\<^esup> Value v"
+      using T1 htrace_to_leaf.intros by simp
+  next
+    fix xs'
+    assume "reg \<turnstile> (t2, v1 # bs, xs) \<Rightarrow>\<^bsup>T2\<^esup>  Tail xs'"
+    then show "reg \<turnstile> (LET t1 IN t2, bs, xs) \<Rightarrow>\<^bsup>T1@T2\<^esup>  Tail xs'"
+      using T1 htrace_to_leaf.intros by simp
+  next
+    fix xs'
+    assume "(f, reg) \<turnstile> (f, [], xs') \<Rightarrow>\<^bsup>z2 - interp_trace reg T2 - 1\<^esup>  v"
+    then show "(f, reg) \<turnstile> (f, [], xs') \<Rightarrow>\<^bsup>z - interp_trace reg (T1 @ T2) - 1\<^esup>  v"
+      using hLet T1 htrace_to_leaf.intros interp_trace_append by simp
+  qed
+next
+  case (hLetBound v bs n a b xs)
+  then have "b \<turnstile> (hLetBound n, bs, xs) \<Rightarrow>\<^bsup> [] \<^esup> Value v" using htrace_to_leaf.intros by simp
+  then show ?case by blast
+next
+  case (hArg v xs n a b bs)
+  then have "b \<turnstile> (hArg n, bs, xs) \<Rightarrow>\<^bsup> [] \<^esup> Value v" using htrace_to_leaf.intros by simp
+  then show ?case by blast
+next
+  case (hNumber a b n bs xs)
+  then have "b \<turnstile> (hNumber n, bs, xs) \<Rightarrow>\<^bsup> [] \<^esup> Value n" using htrace_to_leaf.intros by simp
+  then show ?case by blast
+next
+  case (hIfTrue f reg t1 bs xs z1 v1 t2 z2 v2 z t3)
+  from sem_to_trace_non_tailE hIfTrue.hyps(1) obtain T1 where
+    T1: "reg \<turnstile> (t1,bs,xs) \<Rightarrow>\<^bsup>T1\<^esup> Value v1" "interp_trace reg T1 = z1"
+    using hIfTrue.prems invar.simps by blast
+  from hIfTrue.IH(2) obtain T2 where
+      "(reg \<turnstile> (t2,bs,xs) \<Rightarrow>\<^bsup>T2\<^esup> Value v2) \<or>
+       (\<exists>xs'. reg \<turnstile> (t2,bs,xs) \<Rightarrow>\<^bsup>T2\<^esup> Tail xs' \<and>
+              (f, reg) \<turnstile> (f,[],xs') \<Rightarrow>\<^bsup>z2 - interp_trace reg T2 - 1\<^esup> v2)"
+    using hIfTrue.prems by auto
+  then show ?case proof (rule sem_to_trace_inductionI)
+    assume "reg \<turnstile> (t2,bs,xs) \<Rightarrow>\<^bsup>T2\<^esup> Value v2"
+    then show "reg \<turnstile> (IF t1\<noteq>0 THEN t2 ELSE t3,bs,xs) \<Rightarrow>\<^bsup>T1@T2\<^esup> Value v2"
+      using hIfTrue T1 htrace_to_leaf.intros by simp
+  next
+    fix xs'
+    assume "reg \<turnstile> (t2,bs,xs) \<Rightarrow>\<^bsup>T2\<^esup> Tail xs'"
+    then show "reg \<turnstile> (IF t1\<noteq>0 THEN t2 ELSE t3,bs,xs) \<Rightarrow>\<^bsup>T1@T2\<^esup> Tail xs'"
+      using hIfTrue T1 htrace_to_leaf.intros by simp
+  next
+    fix xs'
+    assume "(f,reg) \<turnstile> (f,[],xs') \<Rightarrow>\<^bsup>z2 - interp_trace reg T2 - 1\<^esup>  v2"
+    then show "(f,reg) \<turnstile> (f,[],xs') \<Rightarrow>\<^bsup>z - interp_trace reg (T1@T2) - 1\<^esup> v2"
+      using hIfTrue T1 htrace_to_leaf.intros interp_trace_append by simp
+  qed
+next
+  case (hIfFalse f reg t1 bs xs z1 v1 t3 z2 v2 z t2)
+  from sem_to_trace_non_tailE hIfFalse.hyps(1) obtain T1 where
+    T1: "reg \<turnstile> (t1,bs,xs) \<Rightarrow>\<^bsup>T1\<^esup> Value v1" "interp_trace reg T1 = z1"
+    using hIfFalse.prems invar.simps by blast
+  from hIfFalse.IH(2) obtain T2 where
+      "(reg \<turnstile> (t3,bs,xs) \<Rightarrow>\<^bsup>T2\<^esup> Value v2) \<or>
+       (\<exists>xs'. reg \<turnstile> (t3,bs,xs) \<Rightarrow>\<^bsup>T2\<^esup> Tail xs' \<and>
+              (f,reg) \<turnstile> (f,[],xs') \<Rightarrow>\<^bsup>z2 - interp_trace reg T2 - 1\<^esup> v2)"
+    using hIfFalse.prems by auto
+  then show ?case proof (rule sem_to_trace_inductionI)
+    assume "reg \<turnstile> (t3,bs,xs) \<Rightarrow>\<^bsup>T2\<^esup> Value v2"
+    then show "reg \<turnstile> (IF t1\<noteq>0 THEN t2 ELSE t3,bs,xs) \<Rightarrow>\<^bsup>T1@T2\<^esup> Value v2"
+      using hIfFalse T1 htrace_to_leaf.intros by simp
+  next
+    fix xs'
+    assume "reg \<turnstile> (t3,bs,xs) \<Rightarrow>\<^bsup>T2\<^esup> Tail xs'"
+    then show "reg \<turnstile> (IF t1\<noteq>0 THEN t2 ELSE t3,bs,xs) \<Rightarrow>\<^bsup>T1@T2\<^esup> Tail xs'"
+      using hIfFalse T1 htrace_to_leaf.intros by simp
+  next
+    fix xs'
+    assume "(f,reg) \<turnstile> (f,[],xs') \<Rightarrow>\<^bsup>z2 - interp_trace reg T2 - 1\<^esup>  v2"
+    then show "(f,reg) \<turnstile> (f,[],xs') \<Rightarrow>\<^bsup>z - interp_trace reg (T1@T2) - 1\<^esup> v2"
+      using hIfFalse T1 htrace_to_leaf.intros interp_trace_append by simp
+  qed
+next
+  case (hCall g T_g reg gr zs ts vs f bs xs v' z')
+  then show ?case sorry (* TODO *)
+next
+  case (hTAIL zs ts vs f reg bs xs z' v' z'')
+  then show ?case sorry
+qed
+
+(* TODO is this better *)
+lemma sem_to_traceE':
+  assumes "invar t"
+  assumes "(f,reg) \<turnstile> (t,bs,xs) \<Rightarrow>\<^bsup>z\<^esup> v"
+  obtains T where "
+    (reg \<turnstile> (t,bs,xs) \<Rightarrow>\<^bsup>T\<^esup> Value v) \<or>
+    (\<exists>xs'. reg \<turnstile> (t,bs,xs) \<Rightarrow>\<^bsup>T\<^esup> Tail xs'
+           \<and> (f,reg) \<turnstile> (f,[],xs') \<Rightarrow>\<^bsup>z - interp_trace reg T - 1\<^esup> v)"
+  using assms sem_to_traceE by blast
+
+lemma sem_to_trace_existsE:
+  assumes "invar t"
+  assumes "(f,reg) \<turnstile> (t,bs,xs) \<Rightarrow>\<^bsup> z \<^esup> v"
+  obtains T :: trace and l where "reg \<turnstile> (t,bs,xs) \<Rightarrow>\<^bsup>T\<^esup> l"
+  using sem_to_traceE assms by blast
+
+(*
+lemma trace_val_from_semantics:
+  assumes "invar t" (* ? *)
   assumes "(f,reg) \<turnstile> (t,bs,xs) \<Rightarrow>\<^bsup> z \<^esup> v1"
-  shows "\<exists>T l. reg \<turnstile> (t,bs,xs) \<Rightarrow>\<^bsup>T\<^esup> l \<and>
-    (case l of
-        Value v2 \<Rightarrow> v2 = v1
-      | Tail xs' \<Rightarrow> (f,reg) \<turnstile> (f,[],xs') \<Rightarrow>\<^bsup>z - interp_trace reg T - 1\<^esup> v)"
+  assumes "reg \<turnstile> (t,bs,xs) \<Rightarrow>\<^bsup>T\<^esup> Value v2"
+  shows "v1 = v2 \<and> interp_trace reg T = z"
   sorry
 
+lemma non_tails_trace: (* useful/meaningful? *)
+  assumes "\<not> tails t"
+  assumes "(f,reg) \<turnstile> (t,bs,xs) \<Rightarrow>\<^bsup> z \<^esup> v"
+  obtains T where "reg \<turnstile> (t,bs,xs) \<Rightarrow>\<^bsup> T \<^esup> Value v" "interp_trace reg T = z"
+  using trace_exists_non_tail trace_val_from_semantics assms no_tails_invar by blast
 
+lemma trace_tail_from_semantics:
+  assumes "invar t" (* ? *)
+  assumes "(f,reg) \<turnstile> (t,bs,xs) \<Rightarrow>\<^bsup> z \<^esup> v"
+  assumes "reg \<turnstile> (t,bs,xs) \<Rightarrow>\<^bsup>T\<^esup> Tail xs'"
+  shows "(f,reg) \<turnstile> (f,[],xs') \<Rightarrow>\<^bsup>z - interp_trace reg T - 1\<^esup> v"
+  sorry
 
+lemma trace_from_semantics:
+  assumes "invar t"
+  assumes "(f,reg) \<turnstile> (t,bs,xs) \<Rightarrow>\<^bsup> z \<^esup> v1"
+  assumes "reg \<turnstile> (t,bs,xs) \<Rightarrow>\<^bsup> T :: trace \<^esup> l"
+  shows "(case l of
+      Value v2 \<Rightarrow> v2 = v1
+    | Tail xs' \<Rightarrow> (f,reg) \<turnstile> (f,[],xs') \<Rightarrow>\<^bsup>z - interp_trace reg T - 1\<^esup> v)"
+  using trace_val_from_semantics[OF assms(1) assms(2)] trace_tail_from_semantics assms sorry
 
-term eval_to_tail
-
-inductive teval_to_tail where
-  "teval_to_tail s tSKIP None" |
-  "teval_to_tail s (tAssign x a) None" |
-  "\<lbrakk> f \<turnstile> (c1,s) \<Rightarrow>\<^bsup>z1\<^esup> s2; teval_to_tail s2 c2 s3 \<rbrakk> \<Longrightarrow> teval_to_tail s (tSeq c1 c2) s3" |
-  "\<lbrakk> s x \<noteq> 0; teval_to_tail s c1 t \<rbrakk> \<Longrightarrow> teval_to_tail s (tIf x c1 c2) t" |
-  "\<lbrakk> s x = 0; teval_to_tail s c2 t \<rbrakk> \<Longrightarrow> teval_to_tail s (tIf x c1 c2) t" |
-  "teval_to_tail s (tCall c x) None" |
-  "teval_to_tail s tTAIL (Some s)"
-
-inductive_cases teval_to_tail_tIfE[elim!]: "teval_to_tail s (tIf x c1 c2) t"
-
-inductive ttime_to_tail :: "state \<Rightarrow> tcom \<Rightarrow> nat \<Rightarrow> bool" where
-  "ttime_to_tail s tSKIP 1" |
-  "ttime_to_tail s (tAssign x a) 2" |
-  "\<lbrakk> f \<turnstile> (c1,s) \<Rightarrow>\<^bsup>z1\<^esup> s2; ttime_to_tail s2 c2 z2; z = z1 + z2 \<rbrakk> \<Longrightarrow> ttime_to_tail s (tSeq c1 c2) z" |
-  "\<lbrakk> s x \<noteq> 0; ttime_to_tail s c1 z; z' = z + 1 \<rbrakk> \<Longrightarrow> ttime_to_tail s (tIf x c1 c2) z'" |
-  "\<lbrakk> s x = 0; ttime_to_tail s c2 z; z' = z + 1 \<rbrakk> \<Longrightarrow> ttime_to_tail s (tIf x c1 c2) z'" |
-  "\<lbrakk> (c,s) \<Rightarrow>\<^bsup>z\<^esup> s2 \<rbrakk> \<Longrightarrow> ttime_to_tail s (tCall c x) z" |
-  "ttime_to_tail s tTAIL 5"
-
-
-lemma tnon_tail_ctxt_swap:
-  fixes f c :: tcom
-  assumes "f \<turnstile> (c,s) \<Rightarrow>\<^bsup>z\<^esup> t"
-  assumes "\<not>tails c"
-  shows "g \<turnstile> (c,s) \<Rightarrow>\<^bsup>z\<^esup> t"
-  using assms apply (induction f "(c,s)" z t arbitrary: c s rule: tbig_step_t.induct) apply simp_all
-       apply blast
-      apply blast
-     apply blast (* TODO *)
-  by auto
-
-theorem ttime_to_tail:
-  fixes c :: tcom
-  assumes "invar c"
-  assumes "f \<turnstile> (c,s1) \<Rightarrow>\<^bsup>z\<^esup> s3"
-  assumes "teval_to_tail s1 c (Some s2)"
-  shows "\<exists>z1 z2. z = z1 + z2 \<and> ttime_to_tail s1 c z1 \<and> f \<turnstile> (f,s2) \<Rightarrow>\<^bsup>z2\<^esup> s3"
-using assms proof (induction c arbitrary: s1 z)
-  case tSKIP
-  then show ?case using teval_to_tail.cases by fastforce
-next
-  case (tAssign x1 x2)
-  then show ?case using teval_to_tail.cases by fastforce
-next
-  case (tSeq c1 c2) (* TODO cleanup *)
-  (* with tnon_tail_ctxt_swap tdeterm show ?case sledgehammer *)
-
-  obtain z11 s'1 z2 where a: "f \<turnstile> (c1,s1) \<Rightarrow>\<^bsup>z11 \<^esup> s'1" and b: "f \<turnstile> (c2,s'1) \<Rightarrow>\<^bsup>z2 \<^esup> s3" and c: "z=z11+z2"
-    using tSeq tSeq_tE by blast
-  thm tSeq.IH(2) tSeq.prems(2)
-
-  have "invar c2" using tSeq by simp
-
-  obtain f' z1 s' where 1: "f' \<turnstile> (c1,s1) \<Rightarrow>\<^bsup>z1\<^esup> s'" and 2: "teval_to_tail s' c2 (Some s2)"
-    using teval_to_tail.cases[OF tSeq.prems(3), simplified] by metis
-  then have "f \<turnstile> (c1,s1) \<Rightarrow>\<^bsup>z1\<^esup> s'" using tnon_tail_ctxt_swap tSeq by simp
-
-  with a tdeterm have d: (* "z1 = z11" *) "s' = s'1" by simp_all
-
-  obtain z1a z2a where "z2 = z1a + z2a \<and> ttime_to_tail s'1 c2 z1a \<and> f \<turnstile> (f, s2) \<Rightarrow>\<^bsup>z2a\<^esup>  s3"
-    using tSeq.IH(2)[OF \<open>invar c2\<close> b 2[simplified d]] by blast
-
-  with a c show ?case by (metis add.assoc ttime_to_tail.intros(3))
-next
-  case (tIf x1 c1 c2) (* TODO cleanup *)
-  then show ?case
-  proof (cases rule: tIf_tE[OF tIf.prems(2)])
-    case (1 x)
-    then show ?thesis
-      by (smt (verit, ccfv_SIG) Suc_eq_plus1 add.assoc add.commute invar.simps(2) not_gr_zero tIf.IH(1) tIf.prems(1,3) teval_to_tail_tIfE
-          ttime_to_tail.intros(4))
-  next
-    case (2 x)
-    then show ?thesis
-      by (smt (verit, ccfv_threshold) Suc_eq_plus1 add.assoc add.commute invar.simps(2) less_numeral_extra(3) tIf.IH(2) tIf.prems(1,3) teval_to_tail_tIfE
-          ttime_to_tail.intros(5))
-  qed
-next
-  case (tCall x1 x2)
-  then show ?case using teval_to_tail.cases by fastforce
-next
-  case tTAIL
-  then obtain z' where z': "z = 5 + z'" "f \<turnstile> (f,s1) \<Rightarrow>\<^bsup>z'\<^esup> s3" using tTail_tE by blast
-  then have "f \<turnstile> (f,s2) \<Rightarrow>\<^bsup>z - 5\<^esup>  s3" using tTAIL teval_to_tail.cases by auto
-  with z' show ?case using ttime_to_tail.intros(7) by auto
-qed
-
-(*
-
-inductive ttime_to_tail where
-  "ttime_to_tail s tSKIP [] (Suc (0::nat))" |
-  "ttime_to_tail s (tAssign x a) [] (Suc (Suc (0::nat)))" |
-  "\<lbrakk> ttime_to_tail s c1 gs1 k1; f \<turnstile> (c1,s) \<Rightarrow>\<^bsup>z1\<^esup> s2; ttime_to_tail s2 c2 gs2 k2; k = k1 + k2 \<rbrakk>
-   \<Longrightarrow> ttime_to_tail s (tSeq c1 c2) (gs1 @ gs2) k" |
-  "\<lbrakk> s x \<noteq> 0; ttime_to_tail s c1 gs k; k' = k + 1 \<rbrakk> \<Longrightarrow> ttime_to_tail s (tIf x c1 c2) gs k'" |
-  "\<lbrakk> s x = 0; ttime_to_tail s c2 gs k; k' = k + 1 \<rbrakk> \<Longrightarrow> ttime_to_tail s (tIf x c1 c2) gs k'" |
-  "ttime_to_tail s (tCall c x) [(c,s)] 0" |
-  "ttime_to_tail s tTAIL [] 5"
-
-definition "tinterp_time gs k z \<equiv>
-  (\<exists>zgs. (\<forall>(zg,(c,s)) \<in> set (zip zgs gs). \<exists>s'. (c,s) \<Rightarrow>\<^bsup>zg\<^esup> s') \<and> z = sum_list zgs + k)"
-
-theorem ttime_to_tail:
-  fixes c :: tcom
-  assumes "invar c"
-  assumes "f \<turnstile> (c,s1) \<Rightarrow>\<^bsup>z\<^esup> s3"
-  assumes "teval_to_tail s c (Some s2)"
-  shows "\<exists>gs k z1 z2. z = z1 + z2 \<and> ttime_to_tail s c gs k \<and> tinterp_time gs k z1 \<and> f \<turnstile> (f,s2) \<Rightarrow>\<^bsup>z2\<^esup> s3"
-using assms proof (induction c arbitrary: s)
 *)
-
-(* assumptions:
-    - variable names of function arguments and return values of
-      called functions and f itself do not conflict
-    - correct number of arguments to call/recurse constructors *)
-
-(* let us switch between definitions easily *)
-abbreviation "fresh' \<equiv> Fresh.fresh"
-
-(*
-definition map_fresh where
-  "map_fresh stale name f xs =
-    snd ((foldl (\<lambda>(st0, xs') x. (fresh' st0 name # st0, xs' @ [f st0 (fresh' st0 name) x])) (stale, [])) xs)"
-
-value "map_fresh [] ''x'' (\<lambda>v vs (x :: nat). (x, v, vs)) [1, 2, 3]"
-
-definition "fresh_n (n :: nat) stale name = snd (fold (\<lambda>_ (st0, r).
-  let x = fresh' st0 name in (x # st0, r @ [(x, st0)])) [1..int n] (stale, []))" *)
-
-(* definition "make_n (n :: nat) name = [name @ string_of_nat i . i <- [0..<n]]" *)
-definition "make_n_fresh n stale name = map (fresh' stale o ((@) name) o string_of_nat) [0..<n]"
-
-lemma distinct_make_n_fresh: "distinct (make_n_fresh n stale name)"
-unfolding make_n_fresh_def proof (subst distinct_map, standard)
-  show "inj_on (fresh' stale \<circ> (@) name \<circ> string_of_nat) (set [0..<n])"
-    using comp_inj_on inj_string_of_nat inj_append2 Fresh.inj_fresh inj_on_subset[where A = UNIV, simplified]
-    by metis
-qed simp
-
-value "make_n_fresh 5 [''f.args.2.0'', ''f.args.2.1'', ''f.args.3.0''] ''f.args.''"
-
-(* definition "foldr1 f xs = foldr f (butlast xs) (last xs)" *)
-(* definition "t_seqs ts = foldr1 tSeq ts" (* (if ts = [] then tSKIP else  *) *)
-definition "t_seqs ts = foldr tSeq ts" (* (if ts = [] then tSKIP else  *)
-value "t_seqs ([c1, c2, c3]) c4"
-
-(* lemma foldr1_append: assumes "xs \<noteq> []" "ys \<noteq> []" shows "foldr1 f (xs @ ys) = foldr tSeq xs (foldr1 tSeq ys)" *)
-
-lemma invar_tseqs[simp]: assumes "\<forall>t \<in> set xs. \<not> tails t" "invar x" shows "invar (t_seqs xs x)"
-  unfolding t_seqs_def using assms by (induction xs) simp_all
-lemma non_tails_tseqs[simp]: assumes "\<forall>t \<in> set xs. \<not> tails t" "\<not> tails x" shows "\<not> tails (t_seqs xs x)"
-  unfolding t_seqs_def using assms by (induction xs) simp_all
-(* lemma non_tails_tseqs_append: assumes "\<not> tails (t_seqs xs)" "\<not> tails (t_seqs ys)" shows "\<not> tails (t_seqs (xs @ ys) x)" *)
-  (* using assms unfolding t_seqs_def foldr1_def apply (induction xs) apply simp_all *)
-  (* apply (cases xs) unfolding t_seqs_def foldr1_def apply simp *)
-  (* apply (cases ys) *)
-  (* apply simp sledgehammer *)
-   (* apply (induction xs) unfolding t_seqs_def foldr1_def apply simp_all *)
-
-abbreviation "mapi f xs \<equiv> snd (fold (\<lambda>x (i, ys). (i + 1, ys @ [f i x])) xs (0, []))"
-
-lemma mapi_map2[simp]: "mapi f xs = map2 f [0..<length xs] xs"
-proof-
-  have gen: "snd (fold (\<lambda>x (i, ys). (i + 1, ys @ [f i x])) xs (length ys, ys))
-             = ys @ map2 f [length ys..<length ys + length xs] xs" for xs ys
-  proof (induction xs arbitrary: ys)
-    case (Cons x xs)
-    have "[length ys..<length ys + length (x # xs)]
-          = length ys # [Suc (length ys)..<length ys + length (x # xs)]"
-      using upt_conv_Cons upt_rec by simp
-    thus ?case using Cons[of "ys @ [f (length ys) x]"] by simp
-  qed simp
-  from gen[where ys = "[]"] show "mapi f xs = map2 f [0..<length xs] xs" by simp
-qed
-
-find_theorems "?t \<in> set (map ?f ?xs)"
-
-lemma map_obtain: assumes "y \<in> set (map f xs)" obtains x where "y = f x" "x \<in> set xs" using assms by auto
-
-lemma mapi_obtain:
-  assumes "y \<in> set (mapi f xs)"
-  obtains i x where "y = f i x" "i < length xs" "x \<in> set xs"
-proof-
-  from assms have "y \<in> set (map2 f [0..<length xs] xs)" by (simp only: mapi_map2)
-  then obtain i1 x1 where 1: "y = f i1 x1" "(i1, x1) \<in> set (zip [0..<length xs] xs)" by auto
-  then have "i1 \<in> set [0..<length xs]" and 3: "x1 \<in> set xs" using in_set_zipE by meson+
-  then have 2: "i1 < length xs" by simp
-  from 1 2 3 show thesis using that[where i = i1 and x = x1] by simp
-qed
-
-
-fun to_imp_tc ::
-    "vname list \<Rightarrow> thol_ctxt
-    \<Rightarrow> vname list \<Rightarrow> vname \<Rightarrow> vname list \<Rightarrow> thol
-    \<Rightarrow> tcom" where
-  (* f_args: list of argument registers' names
-     ctxt: see type def
-     bs: names of bound variables
-     r: return register name
-     stale: variable names that must not be written to *)
-  (* fresh variables: need two conditions:
-    - must not overwrite live variables
-    - must not be overwritten before any use *)
-  "to_imp_tc f_args ctxt bs r stale (hIf t1 t2 t3) =
-    (let x_var = fresh' stale ''If.x'';
-         c1 = to_imp_tc f_args ctxt bs x_var stale t1;
-         c2 = to_imp_tc f_args ctxt bs r stale t2;
-         c3 = to_imp_tc f_args ctxt bs r stale t3
-      in tSeq c1 (tIf x_var c2 c3))" |
-  "to_imp_tc f_args ctxt bs r stale (hLet t1 t2) =
-    (let x_var = fresh' stale ''Let.x'';
-         c1 = to_imp_tc f_args ctxt bs x_var stale t1;
-         c2 = to_imp_tc f_args ctxt (x_var # bs) r (x_var # stale) t2
-      in tSeq c1 c2)" |
-  "to_imp_tc f_args ctxt bs r stale (hLetBound n) = tAssign r (A (V (bs ! n)))" |
-  "to_imp_tc f_args ctxt bs r stale (hArg n) = tAssign r (A (V (f_args ! n)))" |
-  "to_imp_tc f_args ctxt bs r stale (hNumber n) = tAssign r (A (N n))" |
-  (* TODO: call/TAIL cases could be written more nicely, but need termination proofs.
-      On the other hand, this more closely follows the written presentation. *)
-  "to_imp_tc f_args ctxt bs r stale (hCall g ts) =
-    (let (g_args, c_g, g_ret) = ctxt g;
-         xs = make_n_fresh (length ts) stale ''Call.x.'';
-         cs1 = mapi (\<lambda>i t. to_imp_tc f_args ctxt bs (xs ! i) (xs @ stale) t) ts;
-         cs2 = mapi (\<lambda>i t. tAssign (g_args ! i) (A (V (xs ! i)))) ts
-      in t_seqs (cs1 @ cs2) (tSeq (tCall c_g g_ret) (tAssign r (A (V g_ret)))))" |
-  "to_imp_tc f_args ctxt bs r stale (hTAIL ts) =
-    (let xs = make_n_fresh (length ts) stale ''TAIL.x.'';
-         cs1 = mapi (\<lambda>i t. to_imp_tc f_args ctxt bs (xs ! i) (xs @ stale) t) ts;
-         cs2 = mapi (\<lambda>i t. tAssign (f_args ! i) (A (V (xs ! i)))) ts
-      in t_seqs (cs1 @ cs2) tTAIL)"
-
-lemma to_imp_nontail: "non_tail t \<Longrightarrow> \<not> tails (to_imp_tc f_args ctxt bs r stale t)"
-proof (induction t arbitrary: bs r stale)
-  case (hCall g ts)
-  let ?xs = "make_n_fresh (length ts) stale ''Call.x.''"
-  let ?cs1 = "mapi (\<lambda>i t. to_imp_tc f_args ctxt bs (?xs ! i) (?xs @ stale) t) ts"
-  let ?cs2 = "mapi (\<lambda>i t. tAssign (args_from_ctxt ctxt g ! i) (A (V (?xs ! i)))) ts"
-
-  have 1: "\<forall>s \<in> set ?cs1. \<not> tails s"
-  proof
-    fix s
-    assume 1: "s \<in> set ?cs1"
-    obtain i t where "s = to_imp_tc f_args ctxt bs (?xs ! i) (?xs @ stale) t" "t \<in> set ts"
-      using mapi_obtain[OF 1] by blast
-    with hCall show "\<not> tails s" by simp
-  qed
-  have 2: "\<forall>s \<in> set ?cs2. \<not> tails s" apply (subst mapi_map2) apply simp apply (subst split_beta) by simp
-
-  show ?case
-    apply (simp only: to_imp_tc.simps Let_def split_beta)
-    apply (rule non_tails_tseqs) prefer 2 apply simp
-    thm ball_Un
-    apply (simp only: set_append ball_Un, standard)
-    using 1 apply simp using 2 apply simp
-    done
-qed (simp_all add: Let_def) (* why do all the other cases go through by simp ???? TODO: figure it out and clean up these proofs *)
-
-lemma to_imp_invar: "tailrec t \<Longrightarrow> invar (to_imp_tc f_args ctxt bs r stale t)"
-proof (induction t arbitrary: bs r stale)
-  case (hCall g ts)
-  let ?xs = "make_n_fresh (length ts) stale ''Call.x.''"
-  let ?cs1 = "mapi (\<lambda>i t. to_imp_tc f_args ctxt bs (?xs ! i) (?xs @ stale) t) ts"
-  let ?cs2 = "mapi (\<lambda>i t. tAssign (fst (ctxt g) ! i) (A (V (?xs ! i)))) ts"
-
-  have 1: "\<forall>s \<in> set ?cs1. \<not> tails s"
-  proof
-    fix s
-    assume 1: "s \<in> set ?cs1"
-    obtain i t where "s = to_imp_tc f_args ctxt bs (?xs ! i) (?xs @ stale) t" "t \<in> set ts"
-      using mapi_obtain[OF 1] by blast
-    with hCall to_imp_nontail show "\<not> tails s" by simp
-  qed
-  have 2: "\<forall>s \<in> set ?cs2. \<not> tails s" apply (subst mapi_map2) apply simp apply (subst split_beta) by simp
-
-  show ?case
-    apply (simp only: to_imp_tc.simps Let_def split_beta)
-    apply (rule invar_tseqs) prefer 2 apply simp
-    apply (simp only: set_append ball_Un, standard)
-    using 1 apply simp using 2 apply simp
-    done
-next
-  case (hTAIL ts)
-  let ?xs = "make_n_fresh (length ts) stale ''TAIL.x.''"
-  let ?cs1 = "mapi (\<lambda>i t. to_imp_tc f_args ctxt bs (?xs ! i) (?xs @ stale) t) ts"
-  let ?cs2 = "mapi (\<lambda>i t. tAssign (f_args ! i) (A (V (?xs ! i)))) ts"
-
-  have 1: "\<forall>s \<in> set ?cs1. \<not> tails s"
-  proof
-    fix s
-    assume 1: "s \<in> set ?cs1"
-    obtain i t where "s = to_imp_tc f_args ctxt bs (?xs ! i) (?xs @ stale) t" "t \<in> set ts"
-      using mapi_obtain[OF 1] by blast
-    with hTAIL to_imp_nontail show "\<not> tails s" by simp
-  qed
-  have 2: "\<forall>s \<in> set ?cs2. \<not> tails s" apply (subst mapi_map2) apply simp apply (subst split_beta) by simp
-
-  show ?case
-    apply (simp only: to_imp_tc.simps Let_def)
-    apply (rule invar_tseqs) prefer 2 apply simp
-    apply (simp only: set_append ball_Un, standard)
-    using 1 apply simp using 2 apply simp
-    done
-qed (simp_all add: Let_def to_imp_nontail)
-
-(* TODO: rename our tailrec \<rightarrow> h_invar, non_tail \<rightarrow> \<not> h_tails or the likes *)
-
-fun h_calls where
-  "h_calls (hLet t1 t2) = h_calls t1 @ h_calls t2" |
-  "h_calls (hLetBound _) = []" |
-  "h_calls (hArg _) = []" |
-  "h_calls (hNumber _) = []" |
-  "h_calls (hIf t1 t2 t3) = h_calls t1 @ h_calls t2 @ h_calls t3" |
-  "h_calls (hCall f ts) = f # concat (map h_calls ts)" |
-  "h_calls (hTAIL ts) = concat (map h_calls ts)"
-
-definition "reserved_regs f_args ctxt bs t =
-    (f_args @ bs @ concat (map (fst o ctxt) (h_calls t)) @ map (snd o snd o ctxt) (h_calls t))"
-
-(* mark argument/return registers of all called functions and of f itself as stale *)
-definition "to_imp_tc' f_args ctxt bs r t =
-  to_imp_tc f_args ctxt bs r (reserved_regs f_args ctxt bs t) t"
-(* TODO: right-assoc ? *)
-
-definition "h_let_1 = hLet (hNumber 7) (hLetBound 0)"
-value "to_imp_tc_1 [] null ''r'' h_let_1"
-
-definition "h_call_1 = hCall ''g'' [hNumber 7, hNumber 5]"
-value "to_imp_tc_1 [] (null(''g'' := ([''g.x1'', ''g.x2''], Assign ''g.r'' (A (V ''g.x1'')), ''g.r''))) ''r'' h_call_1"
-
-definition "com_plus = ([''plus.x'', ''plus.y''], Assign ''plus.ret'' (Plus (V ''plus.x'') (V ''plus.y'')), ''plus.ret'')"
-definition "h_sum3 = hLet (hCall ''plus'' [hArg 0, hArg 1]) (hCall ''plus'' [hLetBound 0, hArg 2])"
-value "to_imp_tc_1 [''x'', ''y'', ''z''] (null(''plus'' := com_plus)) ''r'' h_sum3"
-
-
-definition "time_thol f reg (t :: thol) vs_b vs_arg z0 = (\<exists>v. \<exists>z. z \<le> z0 \<and> (f,reg) \<turnstile> (t,vs_b,vs_arg) \<Rightarrow>\<^bsup>z\<^esup> v)"
-definition "time_imp c (p :: tcom) s z0 = (\<exists>s'. \<exists>z. z \<le> z0 \<and> c \<turnstile> (p,s) \<Rightarrow>\<^bsup>z\<^esup> s')"
-
-
-definition "t_thol fcs (s's :: state list) = (sum_map (\<lambda>((f_i, _), s'_i). f_i s'_i) (zip fcs s's) :: nat)"
-definition "t_tcom fcs (k :: nat) (s's :: state list) = k + sum_map (\<lambda>((f_i, c_i), s'_i). c_i * f_i s'_i) (zip fcs s's)"
-
-lemma t_thol_sum1: "f s' + t_thol fcs s's = t_thol ((f, c) # fcs) (s' # s's)"
-  unfolding t_thol_def by (simp add: zip_Cons)
-
-(*
-thm list_induct2'
-find_theorems "(\<And>x1 x2 y1 y2. ?P x2 y2 \<Longrightarrow> ?P (x1 # x2) (y1 # y2) )"
-
-lemma t_thol_sum: "t_thol fcs1 s's1 + t_thol fcs2 s's2 = t_thol (fcs1 @ fcs2) (s's1 @ s's2)"
-  unfolding t_thol_def sum_map_def using t_thol_sum1 apply (induction fcs1 s's1 rule: list_induct2')
-  apply simp different lengths... *)
-
-abbreviation "lookups names (s :: state) \<equiv> map s names"
-
-definition "is_call_in t f = (f \<in> set (h_calls t))"
-
-term time_to_tail term ttime_to_tail
-thm time_to_tail ttime_to_tail
-
-
-fun tstruct_k :: "tcom \<Rightarrow> nat" where
-  "tstruct_k tSKIP = 1" |
-  "tstruct_k (tAssign _ _) = 2" |
-  "tstruct_k (tSeq c1 c2) = tstruct_k c1 + tstruct_k c2 + 1" |
-  "tstruct_k (tIf x c1 c2) = max (tstruct_k c1) (tstruct_k c2) + 1" |
-  "tstruct_k (tCall _ _) = 0" |
-  "tstruct_k tTAIL = 5"
-
-
 
 end
